Suppose we can find N dependent constants α_L and α_U such that $\alpha_L <= |\alpha_1(s)| <= \alpha_U$

We can lower bound the summand denominators as $Re(s + (t/2)\alpha_1(s)) \le \sigma + (t/2)\alpha_L$

Among the numerators, we can upper bound different terms as $|2\alpha_1(s) - log(n)| < |2\alpha_1(s)| <= 2\alpha_U$ since |(a + bi) - c| < |a + bi| if a, c > 0 and a > c

$$|\alpha_1^2(s) - \alpha_1^2(1-s)| \le |\alpha_1(s) + \alpha_1(1-s)| |\alpha_1(s) - \alpha_1(1-s)|$$

Now $|\alpha_1(s) + \alpha_1(1-s)| <= 2\alpha_U$

and
$$\alpha_{diff} = |\alpha_1(s) - \alpha_1(1 - s)|$$

 $<= |\frac{3}{2}(\frac{1}{s} + \frac{1}{s-1})| + \frac{1}{2}|\log \frac{s}{1-s}|$
 $<= \frac{3}{x_N} + \frac{1}{2}\log|\frac{1-y+ix}{1+y-ix}| + \frac{1}{2}|i(tan^{-1}(\frac{x}{1-y}) + tan^{-1}(\frac{x}{1+y}))|$
 $<= \frac{3}{x_N} + \frac{1}{4}\log \frac{(1-y)^2 + x_{N+1}^2}{(1+y)^2 + x_N^2} + \frac{\pi}{2}$
 $<= \frac{\pi}{2} + \frac{3}{x_N} + \frac{1}{2}\log \frac{x_{N+1}}{x_N} \text{ since } \frac{a+b}{c+d} < \frac{b}{d} \text{ if } a < c \text{ and } d < b$

(From the wiki, it is possible $|\alpha_1(s) - \alpha_1(1-s)| \le \frac{y}{x_N-6}$ would also work although it was derived from $|\alpha_1(s) - \overline{\alpha_1(1-s)}|$)

$$|\lambda| \le e^{\delta}/N^y$$
 (from the wiki)

$$\begin{split} &\text{So,} \\ &|\frac{d}{dt} \frac{A^{eff} + B^{eff}}{B_0^{eff}}| \\ &<= \frac{1}{4} \sum_{n=1}^{N} \frac{b_n^t |\log^2 n - 2 \log(n) \alpha_1(s_B)|}{n^{Re(s_B + (t/2)\alpha_1(s_B))}} + \frac{|\lambda|}{4} \sum_{n=1}^{N} \frac{b_n^t |\log^2 n - 2 \log(n) \alpha_1(s_A) + \alpha_1^2(s_A) - \alpha_1^2(s_B)|}{n^{Re(s_A + (t/2)\alpha_1(s_A))}} \\ &<= \frac{1}{4} \sum_{n=1}^{N} \frac{2 \alpha_U b_n^t log(n)}{n^{1-\sigma + (t/2)\alpha_L}} + \frac{e^{\delta}}{N^y} \sum_{n=1}^{N} \frac{2 \alpha_U b_n^t (log(n) + 2 \alpha_U \alpha_{diff})}{n^{\sigma + (t/2)\alpha_L}} \\ &<= \frac{\alpha_U}{2} \sum_{n=1}^{N} (\frac{b_n^t log(n)}{n^{1-\sigma + (t/2)\alpha_L}} + \frac{e^{\delta}}{N^y} \frac{b_n^t (log(n) + \alpha_{diff})}{n^{\sigma + (t/2)\alpha_L}}) \\ &\alpha_L = log(N), \alpha_U = log(N) + 1 \text{ works but may not be that tight} \\ &\alpha_L = \frac{1}{2} \log \frac{|1-y + ix_N|}{4\pi}, \alpha_U = \frac{\pi}{4} + \frac{3}{2x_N} + \frac{1}{2} \log \frac{|1+y + ix_N + 1|}{4\pi} \text{ is much tighter} \end{split}$$

To improve the bound further, we can treat $|2\alpha_1(s) - log(n)|$ = $|2(\frac{1}{2s} + \frac{1}{s-1}) + log\frac{s}{2\pi} - log(n)|$ <= $|2(\frac{1}{2s} + \frac{1}{s-1}) + log\frac{|1+y+ix_{N+1}|}{4\pi n} + i\frac{\pi}{2}|$ <= $\frac{\pi}{2} + \frac{3}{x_N} + log\frac{|1+y+ix_{N+1}|}{4\pi n}$ = $2\alpha_U - log(n)$

This gives an improved bound,

$$\begin{split} & \big| \frac{d}{dt} \frac{A^{eff} + B^{eff}}{B_0^{eff}} \big| \\ <& = \frac{1}{4} \sum_{n=1}^N \Big(\frac{b_n^t log(n)(2\alpha_U - \log(n))}{n^{1-\sigma + (t/2)\alpha_L}} + \frac{e^{\delta}}{N^y} \frac{b_n^t (log(n)(2\alpha_U - \log(n)) + 2\alpha_U \alpha_{diff})}{n^{\sigma + (t/2)\alpha_L}} \Big) \end{split}$$